theories/L0_QuotedCoq/term.v
@@ -1,0 +1,505 @@
+
+Add LoadPath "../common" as Common.
+
+Require Export Template.Ast.
+Require Import Coq.Strings.String.
+Require Import Coq.Bool.Bool.
+Require Import Coq.Arith.Peano_dec.
+Require Import Coq.Logic.Eqdep_dec.
+Require Import Coq.Lists.List.
+Require Import Coq.omega.Omega.
+
+Require Import Common.RandyPrelude.
+Require Import Common.exceptionMonad.
+Require Import Common.AstCommon.
+
+Open Scope list_scope.
+Open Scope bool_scope.
+Set Implicit Arguments.
+
+
+(** Check applications are (hereditarily) well-formed,
+*** and omit unused term forms (tVar, ...) **)
+Definition isNotApp (t:term) : bool :=
+  match t with
+    | tApp _ _ => false
+    | _ => true
+  end.
+
+Section termSize_sec.
+  Variable A : Set.
+  Variable termSize: A -> nat.
+  Fixpoint termsSize (ts:list A) : nat :=
+    match ts with
+      | nil => 0
+      | cons r rs => S (termSize r + termsSize rs)
+    end.
+  Fixpoint defsSize (ds: list (def A)) : nat :=
+   match ds with
+     | nil => 0
+     | cons d ds =>
+        2 + (termSize (dtype _ d) + termSize (dbody _ d) + defsSize ds)
+   end.
+End termSize_sec.
+
+Fixpoint termSize (t:term) : nat :=
+  match t with
+    | tProd _ ty bod => S (termSize bod + termSize ty)
+    | tLambda _ ty bod => S (termSize bod + termSize ty)
+    | tLetIn _ dfn ty bod => S (termSize dfn + termSize ty + termSize bod)
+    | tApp fn args => S (termSize fn + termsSize termSize args)
+    | tCase _ ty mch brs =>
+      S (termSize ty + termSize mch +
+         termsSize (fun x => termSize (snd x)) brs)
+    | tFix ds _ => S (defsSize termSize ds)
+    | tCast t _ ty => S (termSize t + termSize ty)
+    | _ => 1
+  end.
+
+Lemma termsSize_map_lem:
+  forall (brs:list (nat * term)),
+    termsSize termSize (map snd brs) =
+    termsSize (fun x : nat * term => termSize (snd x)) brs.
+Proof.
+  induction brs; cbn. reflexivity.
+  rewrite IHbrs. reflexivity.
+Qed.
+
+
+(****** how to do a wf fixpoint ??? ************
+
+Definition wf_terms (wf_term:term -> bool) (bs:list term) : bool :=
+  fold_left (fun (b:bool) (t:term) => andb (wf_term t) b) bs true.
+
+Fixpoint wf_term (t:term) : bool.
+Proof.
+  revert t. apply (wf_rec termSize (fun x:term => bool)). intros t wfih.
+  case_eq t; intros; subst.
+  - exact true.  (* Rel *)
+  - exact false.
+  - exact false.
+  - exact false.
+  - exact true. (* Sort *)
+  - refine (wfih t0 _ && wfih t1 _); cbn; omega.
+  - refine (wfih t0 _ && wfih t1 _); cbn; omega.
+  - refine (wfih t0 _ && wfih t1 _); cbn; omega.
+  - refine (wfih t0 _ && wfih t1 _ && wfih t2 _); cbn; omega.
+  - case_eq l; intros; subst.
+    + exact false.  (* App with no argument *)
+    + refine (wfih t0 _ && wfih t _ && wf_terms wf_term l0); cbn; omega.
+  - exact true.
+  - exact true.
+  - exact true.
+  - refine (wfih t0 _ && wfih t1 _ && wf_terms wf_term (map snd l));
+    cbn. omega. rewrite <- termsSize_map_lem. omega.
+  - exact false.  (* Fix *)
+  - exact false.  (* Unknown *)
+Defined.    
+**************************)
+
+(**********************
+(*** Compute wf_term by well-founded induction on size of terms  ***)
+Definition tts_size (x:term * list term) : nat :=
+  termSize (fst x) + termsSize termSize (snd x).
+
+Function explode_defs (ds:list (def term)) : list term :=
+  match ds with
+    | nil => nil
+    | cons {| dtype:= dty; dbody:= dtm |} es =>
+      dty :: dtm :: (explode_defs es)
+  end.
+
+Lemma abcd_lt_lem:
+  forall a b c d:nat,
+    a < S b -> S (c + S (d + a)) < S (S ( S (c + d + b))).
+Proof.
+  intros a b c d h. omega.
+Qed.
+
+Lemma explode_defs_lt:
+  forall (ds:list (def term)) (m:nat),
+    termsSize termSize (explode_defs ds) < termSize (tFix ds m).
+Proof.
+  intros ds m. functional induction (explode_defs ds).
+  - cbn. omega.
+  - cbn in *. apply abcd_lt_lem. assumption.
+Qed.
+                                       
+Definition bool_list_conjunct (bs:list bool) : bool := fold_left andb bs true.
+
+Definition wf_term : term -> bool.
+Proof.
+  eapply (wf_rec termSize (fun (x:term) => bool))%type.
+  intros t wfih.
+  destruct t; intros; subst.
+  - exact true.  (* Rel *)
+  - exact false.
+  - exact false.
+  - exact false.
+  - exact true. (* Sort *)
+  - refine (wfih t0 _ && wfih t1 _); cbn; omega.
+  - refine (wfih t0 _ && wfih t1 _); cbn; omega.
+  - refine (wfih t0 _ && wfih t1 _); cbn; omega.
+  - refine (wfih t0 _ && wfih t1 _ && wfih t2 _); cbn; omega.
+  - assert (T0:bool).
+    { refine (wfih t0 _). cbn. omega. }
+    assert (args:bool).
+    { match l with
+        | nil => exact false
+        | _ => induction l
+      end.
+      + exact true.
+      + assert (A:bool).
+        { refine (wfih a _). cbn. omega. }
+        apply IHl. intros x h. apply (wfih x). cbn in *. omega. } 
+    refine (isNotApp t0 && T0 && args). 
+  - exact true. (* Const *)
+  - exact true. (* Ind *)
+  - exact true. (* Construct *)
+  - assert (Tp:bool).                                    (* Case *)
+    { refine (wfih t0 _). cbn. omega. }
+    assert (Mch:bool).
+    { refine (wfih t1 _). cbn. omega. }
+    assert (Brs:list bool).
+    { induction l.
+      - exact nil.
+      - assert (A:bool).
+         { refine (wfih (snd a) _). cbn. omega. }
+         apply IHl. intros x h. apply (wfih x). cbn in *. omega. }
+    refine (Tp && Mch &&
+               match Brs with
+                 | nil => false
+                 | _ => bool_list_conjunct Brs
+               end).
+  - assert (Ds:list bool).                      (* Fix *)
+    { induction m.        
+      - exact nil.
+      - assert (D:bool).
+        { refine (wfih (dtype term a) _ && wfih (dbody term a) _);
+          cbn; omega. }
+        apply IHm. intros x h. apply (wfih x). cbn in *. omega. }
+      refine (bool_list_conjunct Ds).
+  - exact false.
+Defined.
+Print wf_term.
+
+Require Import Template.Template.
+Require Import Template.Ast.
+
+Quote Definition t0 := ((fun x:bool => x) true).
+Definition t1 : term :=
+  tApp
+    (tLambda nAnon
+             (tInd (mkInd "Coq.Init.Datatypes.bool" 0)) (tRel 0))
+    (cons (tConstruct (mkInd "Coq.Init.Datatypes.bool" 0) 0) nil).
+Eval cbv in (wf_term t1).
+Definition t2 :=  (** App with no args **)   (**** FAILS!!!! *****)
+  tApp
+    (tLambda (nAnon)
+             (tInd (mkInd "Coq.Init.Datatypes.bool" 0)) (tApp (tRel 0) nil))
+    nil.
+Eval cbv in (wf_term t2).
+Definition t3 :=  (** nested App **)   (**** FAILS!!!! *****)
+  tApp (tApp (tRel 0) nil) nil.
+Eval cbv in (wf_term t3).
+
+
+
+Definition wf_term : (term * list term) -> (bool * list bool).
+Proof.
+  eapply (wf_rec tts_size
+                 (fun (x:term * list term) => (bool * list bool)))%type.
+  intros t wfih.
+  assert (wfih': forall (u:term) (us:list term),
+                tts_size (u, us) < tts_size t -> bool * list bool).
+  { intros u us. apply (wfih (u, us)). }
+  clear wfih. destruct t.
+  case_eq t; intros; subst; split.
+  - exact true.  (* Rel *)
+  - exact nil.
+
+  - exact false.
+  - exact nil.
+  - exact false.
+  - exact nil.
+  - exact false.
+  - exact nil.
+  - exact true. (* Sort *)
+  - exact nil.
+  - assert (T0:bool).
+    { refine (fst (wfih' t0 nil _)). cbn. omega. }
+    assert (T1:bool).
+    { refine (fst (wfih' t1 nil _)). cbn. omega. }
+    exact (T0 && T1).
+  - exact nil.
+  - assert (T0:bool).
+    { refine (fst (wfih' t0 nil _)). cbn. omega. }
+    assert (T1:bool).
+    { refine (fst (wfih' t1 nil _)). cbn. omega. }
+    exact (T0 && T1).
+  - exact nil.
+  - assert (T0:bool).
+    { refine (fst (wfih' t0 nil _)). cbn. omega. }
+    assert (T1:bool).
+    { refine (fst (wfih' t1 l _)). cbn. omega. }
+    exact (T0 && T1).
+  - exact nil.
+  - assert (T0:bool).
+    { refine (fst (wfih' t0 nil _)). cbn. omega. }
+    assert (T1:bool).
+    { refine (fst (wfih' t1 nil _)). cbn. omega. }
+    assert (T2:bool).
+    { refine (fst (wfih' t2 nil _)). cbn. omega. }
+    exact (T0 && T1 && T2).
+  - exact nil.
+  - assert (T0:bool).        (* App *)
+    { refine (fst (wfih' t0 nil _)). cbn. omega. }
+    case_eq l0; intros; subst.
+    + exact false.           (* App with nil arg list *)
+    + assert (arg:bool).
+    { refine (fst (wfih' t nil _)). cbn. omega. }
+    assert (args: list bool).
+    { refine (snd (wfih' t l1 _)). cbn. omega. }
+    exact (isNotApp t0 && T0 && arg && bool_list_conjunct args).
+  - exact nil.
+  - exact true.
+  - exact nil.
+  - exact true.
+  - exact nil.
+  - exact true.
+  - exact nil.
+  - assert (T0:bool).   (** case **)
+    { refine (fst (wfih' t0 nil _)). cbn. omega. }
+    assert (T1:bool).
+    { refine (fst (wfih' t1 nil _)). cbn. omega. }
+    assert (brs: list bool).
+    { refine (snd (wfih' t0 (map snd l0) _)). cbn.
+      rewrite <- termsSize_map_lem.
+      omega. }
+    exact (T0 && T1 && bool_list_conjunct brs).
+  - exact nil.
+  - assert (j:= explode_defs_lt m n). cbn in j.    (* Fix *)
+    assert (j0:= (wfih' (tFix m n) (explode_defs m))).
+    assert (T:bool). 
+    { refine (bool_list_conjunct (snd (wfih' (tFix m n) (explode_defs m) _))).
+      cbn in *. apply explode_defs_lt.
+
+    
+  - exact true.    (* Fix **)
+  - exact nil.
+  - exact false.
+  - exact nil.
+Defined.
+
+
+Definition wf_term : (term -> bool).
+Proof.
+  apply (wf_rec termSize (fun x:term => bool)). intros t wfih.
+  case_eq t; intros; subst.
+  - exact true.  (* Rel *)
+  - exact false.
+  - exact false.
+  - exact false.
+  - exact true. (* Sort *)
+  - refine (wfih t0 _ && wfih t1 _); cbn; omega.
+  - refine (wfih t0 _ && wfih t1 _); cbn; omega.
+  - refine (wfih t0 _ && wfih t1 _); cbn; omega.
+  - refine (wfih t0 _ && wfih t1 _ && wfih t2 _); cbn; omega.
+  - destruct l.
+    + exact false.  (* App with no argument *)
+    +
+   
+Defined.
+ *************************)
+
+Function WF_term (n:nat) (t:term) : bool :=
+  match n with
+    | 0 => false
+    | S n => match t with
+               | tRel n => true
+               | tSort srt => true
+               | tCast tm ck ty => WF_term n ty && WF_term n tm
+               | tProd nm ty bod => WF_term n ty && WF_term n bod
+               | tLambda nm ty bod => WF_term n ty && WF_term n bod
+               | tLetIn nm dfn ty bod =>
+                 WF_term n dfn && WF_term n ty && WF_term n bod
+               | tApp fn (cons u us) =>
+                 isNotApp fn &&
+                 WF_term n fn && WF_term n u && WF_terms n us
+               | tConst pth => true
+               | tInd ind => true
+               | tConstruct ind m => true
+               | tCase npars ty mch brs =>
+                 WF_term n ty && WF_term n mch && WF_terms n (map snd brs)
+               | tFix defs m => WF_defs n defs
+               | _ => false
+             end
+  end
+with WF_terms (n:nat) (ts:list term) : bool :=
+       match n with
+         | 0 => false
+         | S n => match ts with
+                    | nil => true
+                    | cons b bs => WF_term n b && WF_terms n bs
+                  end
+       end
+with WF_defs (n:nat) (ds:list (def term)) : bool :=
+       match n with
+         | 0 => false
+         | S n => match ds with
+                    | nil => true
+                    | cons c cs =>
+                      WF_term n (dtype _ c) && WF_term n (dbody _ c) &&
+                              WF_defs n cs
+                  end
+       end.
+Functional Scheme WF_term_ind' := Induction for WF_term Sort Prop
+with WF_terms_ind' := Induction for WF_terms Sort Prop
+with WF_defs_ind' := Induction for WF_defs Sort Prop.
+Combined Scheme WF_term_terms_defs_ind
+         from WF_term_ind', WF_terms_ind', WF_defs_ind'.
+
+Lemma pre_WF_term_up:
+  forall m,
+  (forall t, WF_term m t = true -> WF_term (S m) t = true) /\
+  (forall ts, WF_terms m ts = true -> WF_terms (S m) ts = true) /\
+  (forall ds, WF_defs m ds = true -> WF_defs (S m) ds = true).
+Proof.
+  apply (WF_term_terms_defs_ind
+           (fun (m:nat) (t:term) (q:bool) =>
+              WF_term m t = true -> WF_term (S m) t = true)
+           (fun (m:nat) (ts:list term) (q:bool) =>
+              WF_terms m ts = true -> WF_terms (S m) ts = true)
+           (fun (m:nat) (ds:list (def term)) (q:bool) =>
+              WF_defs m ds = true -> WF_defs (S m) ds = true));
+  intros; intuition; try contradiction.
+  - cbn in H1. destruct (proj1 (andb_true_iff _ _) H1) as [j1 j2].
+    change (WF_term (S n0) ty && WF_term (S n0) tm = true). intuition.
+  - cbn in H1. destruct (proj1 (andb_true_iff _ _) H1) as [j1 j2]. 
+    change (WF_term (S n0) ty && WF_term (S n0) bod = true). intuition.
+  - cbn in H1. destruct (proj1 (andb_true_iff _ _) H1) as [j1 j2]. 
+    change (WF_term (S n0) ty && WF_term (S n0) bod = true). intuition.
+  - cbn in H2.
+    destruct (proj1 (andb_true_iff _ _) H2) as [z1 k3].
+    destruct (proj1 (andb_true_iff _ _) z1) as [k1 k2].
+    change
+      (WF_term (S n0) dfn && WF_term (S n0) ty && WF_term (S n0) bod = true).
+    intuition.
+  - cbn in H2.
+    destruct (proj1 (andb_true_iff _ _) H2) as [z1 k4].
+    destruct (proj1 (andb_true_iff _ _) z1) as [z2 k3].
+    destruct (proj1 (andb_true_iff _ _) z2) as [k1 k2].
+    change (isNotApp fn && WF_term (S n0) fn && WF_term (S n0) u &&
+                     WF_terms (S n0) us = true).
+    rewrite k1. intuition.
+  - cbn in H2.
+    destruct (proj1 (andb_true_iff _ _) H2) as [z1 k3].
+    destruct (proj1 (andb_true_iff _ _) z1) as [k1 k2].
+    change (WF_term (S n0) ty && WF_term (S n0) mch &&
+            WF_terms (S n0) (map snd brs) = true).
+    intuition.
+  - subst. destruct _x; try contradiction; cbn in H; try discriminate.
+    destruct l. discriminate. contradiction.
+  - subst. cbn in H1. destruct (proj1 (andb_true_iff _ _) H1) as [k2 k1].
+    cbn. intuition.
+  - subst. cbn in H2.
+    destruct (proj1 (andb_true_iff _ _) H2) as [z1 k3].
+    destruct (proj1 (andb_true_iff _ _) z1) as [k1 k2].
+    cbn. intuition.
+Qed.
+
+Lemma WF_term_up:
+  forall m t,
+    WF_term m t = true -> forall n, m <= n -> WF_term n t = true.
+Proof.
+  intros m t hm n hn. induction hn.
+  - assumption.
+  - apply (proj1 (pre_WF_term_up m0)). assumption.
+Qed.
+
+Lemma WF_terms_up:
+  forall m ts,
+    WF_terms m ts = true -> forall n, m <= n -> WF_terms n ts = true.
+Proof.
+  intros m ts hm n hn. induction hn.
+  - assumption.
+  - apply (proj1 (proj2 (pre_WF_term_up m0))). assumption.
+Qed.
+
+Lemma WF_defs_up:
+  forall m ds,
+    WF_defs m ds = true -> forall n, m <= n -> WF_defs n ds = true.
+Proof.
+  intros m ds hm n hn. induction hn.
+  - assumption.
+  - apply (proj2 (proj2 (pre_WF_term_up m0))). assumption.
+Qed.
+
+
+(********************************
+Lemma termSize_enough:
+  forall n,
+    (forall t,
+       WF_term n t = true -> WF_term (termSize t) t = true) /\
+    (forall ts,
+       WF_terms n ts = true -> WF_terms (termsSize termSize ts) ts = true) /\
+    (forall ds,
+       WF_defs n ds = true -> WF_defs (defsSize termSize ds) ds = true).   
+Proof.
+  apply (WF_term_terms_defs_ind
+           (fun (m:nat) (t:term) (q:bool) =>
+              WF_term m t = true -> WF_term (termSize t) t = true)
+           (fun (m:nat) (ts:list term) (q:bool) =>
+              WF_terms m ts = true ->
+              WF_terms (termsSize termSize ts) ts = true)
+           (fun (m:nat) (ds:list (def term)) (q:bool) =>
+              WF_defs m ds = true ->
+              WF_defs (defsSize termSize ds) ds = true));
+  intros; intuition; try contradiction.
+  - cbn in *. destruct (andb_true_true _ _ H1).
+    apply (true_true_andb). 
+    + eapply WF_term_up. eapply H. eassumption. omega.
+    + eapply WF_term_up. eapply H0. eassumption. omega.
+  - cbn in *. destruct (andb_true_true _ _ H1).
+    apply (true_true_andb). 
+    + eapply WF_term_up. eapply H. eassumption. omega.
+    + eapply WF_term_up. eapply H0. eassumption. omega.
+  - cbn in *. destruct (andb_true_true _ _ H1).
+    apply (true_true_andb). 
+    + eapply WF_term_up. eapply H. eassumption. omega.
+    + eapply WF_term_up. eapply H0. eassumption. omega.
+  - cbn in *. destruct (andb_true_true _ _ H2).
+    apply (true_true_andb). apply (true_true_andb). 
+    + eapply WF_term_up. eapply H. eassumption. omega.
+    + eapply WF_term_up. eapply H0. eassumption. omega.     
+  - destruct H1. split.
+    * refine (WF_term_up _ _ _). eapply H. assumption. omega.
+    * refine (WF_term_up _ _ _). eapply H0. assumption. omega.
+  - destruct H1. split.
+    * refine (WF_term_up _ _ _). eapply H. assumption. omega.
+    * refine (WF_term_up _ _ _). eapply H0. assumption. omega.
+  - destruct H2 as [j1 [j2 j3]]. repeat split.
+    * refine (WF_term_up _ _ _). eapply H. assumption. omega.
+    * refine (WF_term_up _ _ _). eapply H0. assumption. omega.
+    * refine (WF_term_up _ _ _). eapply H1. assumption. omega.
+  - destruct H2 as [j1 [j2 [j3 j4]]]. repeat split. assumption.
+    * refine (WF_term_up _ _ _). eapply H. assumption. omega.
+    * cbn. refine (WF_term_up _ _ _). eapply H0. assumption. omega.
+    * cbn. refine (WF_terms_up _ _ _). eapply H1. assumption. omega.
+  - destruct H2 as [j1 [j2 j3]]. repeat split.
+    * refine (WF_term_up _ _ _). eapply H. assumption. omega.
+    * refine (WF_term_up _ _ _). eapply H0. assumption. omega.
+    * refine (WF_terms_up _ _ _). eapply H1. assumption. induction brs.
+      + cbn. omega.
+      + cbn. rewrite termsSize_map_lem. omega.
+  - subst. destruct _x; try contradiction.
+    destruct l; try contradiction.
+  - subst. destruct H1. cbn. intuition.
+    + refine (WF_term_up _ _ _). eassumption. omega.
+    + refine (WF_terms_up _ _ _). eassumption. omega.
+  - subst. destruct H2 as [j1 [j2 j3]]. cbn. repeat split.
+    + refine (WF_term_up _ _ _). apply H. eassumption. omega.
+    + refine (WF_term_up _ _ _). apply H0. eassumption. omega.
+    + refine (WF_defs_up _ _ _). apply H1. eassumption. omega.
+Qed.
+*******************************)
